Std/Data/Array/Lemmas.lean
@@ -107,6 +107,9 @@ theorem get_set (a : Array α) (i : Fin a.size) (j : Nat) (hj : j < a.size) (v :
     (a.set i v)[j]'(by simp [*]) = if i = j then v else a[j] := by
   if h : i.1 = j then subst j; simp [*] else simp [*]
 
+theorem set_set (a : Array α) (i : Fin a.size) (v v' : α) :
+    (a.set i v).set ⟨i, by simp [i.2]⟩ v' = a.set i v' := by simp [set, List.set_set]
+
 private theorem fin_cast_val (e : n = n') (i : Fin n) : e ▸ i = ⟨i.1, e ▸ i.2⟩ := by cases e; rfl
 
 theorem swap_def (a : Array α) (i j : Fin a.size) :
